pcuic/theories/PCUICInst.v
@@ -1,0 +1,757 @@
+
+(* Distributed under the terms of the MIT license. *)
+From Coq Require Import Morphisms.
+From MetaCoq.Template Require Import config utils.
+From MetaCoq.PCUIC Require Import PCUICAst PCUICAstUtils PCUICCases PCUICInduction
+  PCUICLiftSubst PCUICUnivSubst PCUICTyping PCUICClosed PCUICEquality PCUICWeakeningEnv
+  PCUICRename.
+
+Require Import ssreflect ssrbool.
+From Equations Require Import Equations.
+Require Import Equations.Prop.DepElim.
+Set Equations With UIP.
+Set Keyed Unification.
+Set Default Goal Selector "!".
+
+(** * Type preservation for σ-calculus instantiation *)
+
+Open Scope sigma_scope.
+
+Definition inst_context σ (Γ : context) : context :=
+  fold_context (fun i => inst (⇑^i σ)) Γ.
+  
+Definition inst_decl σ d := map_decl (inst σ) d.
+
+Definition inst_context_snoc0 s Γ d :
+  inst_context s (d :: Γ) =
+  inst_context s Γ ,, map_decl (inst (⇑^#|Γ| s)) d.
+Proof. unfold inst_context. now rewrite fold_context_snoc0. Qed.
+Hint Rewrite inst_context_snoc0 : sigma.
+
+Lemma inst_context_snoc s Γ d : inst_context s (Γ ,, d) = inst_context s Γ ,, map_decl (inst (⇑^#|Γ| s)) d.
+Proof.
+  unfold snoc. apply inst_context_snoc0.
+Qed.
+Hint Rewrite inst_context_snoc : sigma.
+
+Lemma inst_context_alt s Γ :
+  inst_context s Γ =
+  mapi (fun k' d => map_decl (inst (⇑^(Nat.pred #|Γ| - k') s)) d) Γ.
+Proof.
+  unfold inst_context. apply fold_context_alt.
+Qed.
+
+Lemma inst_context_length s Γ : #|inst_context s Γ| = #|Γ|.
+Proof. apply fold_context_length. Qed.
+Hint Rewrite inst_context_length : sigma wf.
+
+Lemma inst_mkApps f l σ : (mkApps f l).[σ] = mkApps f.[σ] (map (inst σ) l).
+Proof.
+  induction l in f |- *; simpl; auto. rewrite IHl.
+  now autorewrite with sigma.
+Qed.
+Hint Rewrite inst_mkApps : sigma.
+
+Lemma lift0_inst n t : lift0 n t = t.[↑^n].
+Proof. by rewrite lift_rename rename_inst lift_renaming_0 -ren_shiftk. Qed.
+Hint Rewrite lift0_inst : sigma.
+
+Lemma rename_decl_inst_decl :
+  forall f d,
+    rename_decl f d = inst_decl (ren f) d.
+Proof.
+  intros f d.
+  unfold rename_decl, inst_decl.
+  destruct d. unfold map_decl.
+  autorewrite with sigma.
+  f_equal.
+  simpl. destruct decl_body.
+  - simpl. f_equal. autorewrite with sigma. reflexivity.
+  - reflexivity.
+Qed.
+Hint Rewrite rename_decl_inst_decl : sigma.
+
+Lemma rename_context_inst_context :
+  forall f Γ,
+    rename_context f Γ = inst_context (ren f) Γ.
+Proof.
+  intros f Γ.
+  induction Γ.
+  - reflexivity.
+  - autorewrite with sigma. rewrite IHΓ. f_equal.
+    destruct a. unfold inst_decl. unfold map_decl. simpl.
+    f_equal.
+    + destruct decl_body. 2: reflexivity.
+      simpl. f_equal. autorewrite with sigma.
+      now rewrite -up_Upn ren_shiftn.
+    + autorewrite with sigma.
+      now rewrite -up_Upn ren_shiftn.
+Qed.
+Hint Rewrite rename_context_inst_context : sigma.
+
+Lemma subst1_inst :
+forall t n u,
+  t{ n := u } = t.[⇑^n (u ⋅ ids)].
+Proof.
+intros t n u.
+unfold subst1. rewrite subst_inst.
+eapply inst_ext. intro i.
+unfold Upn, subst_compose, subst_consn.
+destruct (Nat.ltb_spec0 i n).
+- rewrite -> nth_error_idsn_Some by assumption. reflexivity.
+- rewrite -> nth_error_idsn_None by lia.
+  rewrite idsn_length.
+  destruct (Nat.eqb_spec (i - n) 0).
+  + rewrite e. simpl. reflexivity.
+  + replace (i - n) with (S (i - n - 1)) by lia. simpl.
+    destruct (i - n - 1) eqn: e.
+    * simpl. reflexivity.
+    * simpl. reflexivity.
+Qed.
+(* Hint Rewrite @subst1_inst : sigma. *)
+
+Lemma subst10_inst a b τ : b {0 := a}.[τ] = (b.[⇑ τ] {0 := a.[τ]}).
+Proof.
+  unfold subst10. simpl. rewrite !subst_inst.
+  now unfold Upn, Up; autorewrite with sigma.
+Qed.
+Hint Rewrite subst10_inst : sigma.
+
+Lemma inst_closed0 σ t : closedn 0 t -> t.[σ] = t.
+Proof. intros. rewrite -{2}[t](inst_closed σ 0) //. now sigma. Qed.
+
+Lemma inst_ext_closed s s' k t : 
+  closedn k t -> 
+  (forall x, x < k -> s x = s' x) -> 
+  inst s t = inst s' t.
+Proof.
+  clear.
+  intros clt Hs. revert k clt s s' Hs.
+  elim t using PCUICInduction.term_forall_list_ind; simpl in |- *; intros; try easy ;
+    try (try rewrite H; try rewrite H0 ; try rewrite H1 ; easy);
+    try solve [f_equal; solve_all].
+  - apply Hs. now eapply Nat.ltb_lt. 
+  - move/andb_and: clt => []. intros. f_equal; eauto.
+    eapply H0; eauto. intros. eapply up_ext_closed; eauto.
+  - move/andb_and: clt => []. intros. f_equal; eauto. now eapply H0, up_ext_closed.
+  - move/andb_and: clt => [] /andb_and[] ?. intros. f_equal; eauto.
+    now eapply H1, up_ext_closed.
+  - move/andb_and: clt => [] ? ?. f_equal; eauto.
+  - move/andb_and: clt => [] /andb_and[] /andP /= [ppars pret] cc b1.
+    red in X. f_equal; eauto.
+    * unfold test_predicate in *. simpl in *. destruct X. solve_all.
+      eapply e; eauto. intros. eapply up_ext_closed; eauto.
+    * eapply All_map_eq. red in X0. solve_all.
+      unfold map_branch. f_equal. now eapply a0, up_ext_closed.
+  - f_equal; eauto. red in X. solve_all.
+    move/andb_and: b => []. eauto. intros.
+    apply map_def_eq_spec; eauto.
+    eapply b0; eauto. now apply up_ext_closed.
+  - f_equal; eauto. red in X. solve_all.
+    move/andb_and: b => []. eauto. intros.
+    apply map_def_eq_spec; eauto.
+    eapply b0; eauto. now apply up_ext_closed.
+Qed.
+
+Lemma subst_id s Γ t : 
+  closedn #|s| t ->
+  assumption_context Γ ->
+  s = List.rev (to_extended_list Γ) ->
+  subst s 0 t = t.
+Proof.
+  intros cl ass eq.
+  autorewrite with sigma.
+  rewrite -{2}(subst_ids t).
+  eapply inst_ext_closed; eauto.
+  intros.
+  unfold ids, subst_consn. simpl.
+  destruct (snd (nth_error_Some' s x) H). rewrite e.
+  subst s.
+  rewrite /to_extended_list /to_extended_list_k in e.
+  rewrite List.rev_length in cl, H. autorewrite with len in *.
+  rewrite reln_alt_eq in e.
+  rewrite app_nil_r List.rev_involutive in e.
+  clear -ass e. revert e.
+  rewrite -{2}(Nat.add_0_r x).
+  generalize 0.
+  induction Γ in x, ass, x0 |- * => n. 
+  - simpl in *. rewrite nth_error_nil => //.
+  - depelim ass; simpl.
+    destruct x; simpl in *; try congruence.
+    move=> e; specialize (IHΓ ass); simpl in e.
+    specialize (IHΓ _ _ _ e). subst x0. f_equal. lia.
+Qed.
+
+Lemma map_inst_idsn l l' n :
+  #|l| = n ->
+  map (inst (l ⋅n l')) (idsn n) = l.
+Proof.
+  induction n in l, l' |- *.
+  - destruct l => //.
+  - destruct l as [|l a] using rev_case => // /=.
+    rewrite app_length /= Nat.add_1_r => [=].
+    intros; subst n.
+    simpl. rewrite map_app.
+    f_equal; auto.
+    + rewrite subst_consn_app.
+      now apply IHn.
+    + simpl.
+      destruct (@subst_consn_lt _ (l ++ [a]) #|l|) as [a' [hnth heq]].
+      * rewrite app_length. simpl; lia.
+      * rewrite heq. rewrite nth_error_app_ge in hnth; auto.
+        rewrite Nat.sub_diag in hnth. simpl in hnth. congruence.
+Qed.
+
+Lemma inst_decl_closed :
+  forall σ k d,
+    closed_decl k d ->
+    inst_decl (⇑^k σ) d = d.
+Proof.
+  intros σ k d.
+  case: d => na [body|] ty. all: rewrite /closed_decl /inst_decl /map_decl /=.
+  - move /andb_and => [cb cty]. rewrite !inst_closed //.
+  - move => cty. rewrite !inst_closed //.
+Qed.
+
+Lemma closed_tele_inst :
+  forall σ ctx,
+    closed_ctx ctx ->
+    mapi (fun i decl => inst_decl (⇑^i σ) decl) (List.rev ctx) =
+    List.rev ctx.
+Proof.
+  intros σ ctx.
+  rewrite /closedn_ctx /mapi. simpl. generalize 0.
+  induction ctx using rev_ind; try easy.
+  move => n.
+  rewrite /closedn_ctx !rev_app_distr /id /=.
+  move /andb_and => [closedx Hctx].
+  rewrite inst_decl_closed //.
+  f_equal. now rewrite IHctx.
+Qed.
+
+Lemma inst_closedn_ctx f n Γ : 
+  closedn_ctx n Γ -> 
+  inst_context (⇑^n f) Γ = Γ.
+Proof.
+  unfold closedn_ctx, rename_context.
+  apply alli_fold_context.
+  intros. rewrite -Upn_Upn Nat.add_comm.
+  now rewrite [map_decl _ _]inst_decl_closed.
+Qed.
+
+Lemma typed_inst :
+  forall Σ Γ t T k σ,
+    wf Σ.1 ->
+    k >= #|Γ| ->
+    Σ ;;; Γ |- t : T ->
+    T.[⇑^k σ] = T /\ t.[⇑^k σ] = t.
+Proof.
+  intros Σ Γ t T k σ hΣ hk h.
+  apply typing_wf_local in h as hΓ.
+  apply typecheck_closed in h. all: eauto.
+  destruct h as [_ [hclΓ hcl]].
+  rewrite -> andb_and in hcl. destruct hcl as [clt clT].
+  pose proof (closed_upwards k clt) as ht.
+  pose proof (closed_upwards k clT) as hT.
+  forward ht by lia.
+  forward hT by lia.
+  rewrite !inst_closed. all: auto.
+Qed.
+
+Lemma inst_wf_local :
+  forall Σ Γ σ,
+    wf Σ.1 ->
+    wf_local Σ Γ ->
+    inst_context σ Γ = Γ.
+Proof.
+  intros Σ Γ σ hΣ h.
+  induction h.
+  - reflexivity.
+  - unfold inst_context, snoc. rewrite fold_context_snoc0.
+    unfold snoc. f_equal. all: auto.
+    unfold map_decl. simpl. unfold vass. f_equal.
+    destruct t0 as [s ht]. eapply typed_inst. all: eauto.
+  - unfold inst_context, snoc. rewrite fold_context_snoc0.
+    unfold snoc. f_equal. all: auto.
+    unfold map_decl. simpl. unfold vdef. f_equal.
+    + f_equal. eapply typed_inst. all: eauto.
+    + eapply typed_inst in t1 as [? _]. all: eauto.
+Qed.
+
+Definition inst_mutual_inductive_body σ m :=
+  map_mutual_inductive_body (fun i => inst (⇑^i σ)) m.
+
+Lemma inst_declared_minductive :
+  forall Σ cst decl σ,
+    wf Σ ->
+    declared_minductive Σ cst decl ->
+    inst_mutual_inductive_body σ decl = decl.
+Proof.
+Admitted.
+(*
+  unfold declared_minductive.
+  intros Σ cst decl σ hΣ h.
+  eapply lookup_on_global_env in h ; eauto. simpl in h.
+  destruct h as [Σ' [hΣ' decl']].
+  destruct decl as [fi npars params bodies univs]. simpl. f_equal.
+  - eapply inst_wf_local. all: eauto.
+    eapply onParams in decl'. auto.
+  - apply onInductives in decl'.
+    revert decl'. generalize bodies at 2 4 5. intros bodies' decl'.
+    eapply Alli_mapi_id in decl'. all: eauto.
+    clear decl'. intros n [na ty ke ct pr] hb. simpl.
+    destruct (decompose_prod_assum [] ty) as [c t] eqn:e1.
+    destruct (decompose_prod_assum [] ty.[⇑^0 σ]) as [c' t'] eqn:e2.
+    destruct hb as [indices s arity_eq onAr csorts onConstr onProj sorts].
+    simpl in *.
+    assert (e : ty.[⇑^0 σ] = ty).
+    { destruct onAr as [s' h'].
+      eapply typed_inst in h' as [_ ?]. all: eauto.
+    }
+    rewrite e in e2. rewrite e1 in e2.
+    revert e2. intros [= <- <-].
+    rewrite e. f_equal.
+    + eapply All_map_id. eapply All2_All_left; tea.
+      intros [[x p] n'] y [[?s Hty] [cs Hargs]].
+      unfold on_pi2; cbn; f_equal; f_equal.
+      eapply typed_inst. all: eauto.
+    + destruct (eq_dec pr []) as [hp | hp]. all: subst. all: auto.
+      specialize (onProj hp).
+      apply on_projs in onProj.
+      apply (Alli_map_id onProj).
+      intros n1 [x p]. unfold on_projection. simpl.
+      intros [? hty].
+      unfold on_snd. simpl. f_equal.
+      eapply typed_inst. all: eauto.
+      simpl.
+      rewrite smash_context_length context_assumptions_fold.
+      simpl. auto.
+Qed.*)
+
+Lemma inst_declared_inductive :
+  forall Σ ind mdecl idecl σ,
+    wf Σ ->
+    declared_inductive Σ ind mdecl idecl ->
+    map_one_inductive_body
+      (context_assumptions mdecl.(ind_params))
+      #|arities_context mdecl.(ind_bodies)|
+      (fun i => inst (⇑^i σ))
+      ind.(inductive_ind)
+      idecl
+    = idecl.
+Proof.
+  intros Σ ind mdecl idecl σ hΣ [hmdecl hidecl].
+  eapply inst_declared_minductive with (σ := σ) in hmdecl. all: auto.
+  unfold inst_mutual_inductive_body in hmdecl.
+  destruct mdecl as [fi npars params bodies univs]. simpl in *.
+  injection hmdecl. intro e. clear hmdecl.
+  pose proof hidecl as hidecl'.
+  rewrite <- e in hidecl'.
+  rewrite nth_error_mapi in hidecl'.
+  clear e.
+  unfold option_map in hidecl'. rewrite hidecl in hidecl'.
+  congruence.
+Qed.
+
+Lemma inst_destArity :
+  forall ctx t σ args s,
+    destArity ctx t = Some (args, s) ->
+    destArity (inst_context σ ctx) t.[⇑^#|ctx| σ] =
+    Some (inst_context σ args, s).
+Proof.
+  intros ctx t σ args s h.
+  induction t in ctx, σ, args, s, h |- * using term_forall_list_ind.
+  all: simpl in *. all: try discriminate.
+  - inversion h. reflexivity.
+  - erewrite <- IHt2 ; try eassumption.
+    simpl. autorewrite with sigma. reflexivity.
+  - erewrite <- IHt3. all: try eassumption.
+    simpl. autorewrite with sigma. reflexivity.
+Qed.
+
+
+(* Lemma types_of_case_rename : *)
+(*   forall Σ ind mdecl idecl npar args u p pty indctx pctx ps btys f, *)
+(*     wf Σ -> *)
+(*     declared_inductive Σ ind mdecl idecl -> *)
+(*     types_of_case ind mdecl idecl (firstn npar args) u p pty = *)
+(*     Some (indctx, pctx, ps, btys) -> *)
+(*     types_of_case *)
+(*       ind mdecl idecl *)
+(*       (firstn npar (map (rename f) args)) u (rename f p) (rename f pty) *)
+(*     = *)
+(*     Some ( *)
+(*         rename_context f indctx, *)
+(*         rename_context f pctx, *)
+(*         ps, *)
+(*         map (on_snd (rename f)) btys *)
+(*     ). *)
+(* Proof. *)
+(*   intros Σ ind mdecl idecl npar args u p pty indctx pctx ps btys f hΣ hdecl h. *)
+(*   unfold types_of_case in *. *)
+(*   case_eq (instantiate_params (subst_instance_context u (ind_params mdecl)) (firstn npar args) (subst_instance_constr u (ind_type idecl))) ; *)
+(*     try solve [ intro bot ; rewrite bot in h ; discriminate h ]. *)
+(*   intros ity eity. rewrite eity in h. *)
+(*   pose proof (on_declared_inductive hΣ as hdecl) [onmind onind]. *)
+(*   apply onParams in onmind as Hparams. *)
+(*   assert (closedparams : closed_ctx (subst_instance_context u (ind_params mdecl))). *)
+(*   { rewrite closedn_subst_instance_context. *)
+(*     eapply PCUICWeakening.closed_wf_local. all: eauto. eauto. } *)
+(*   epose proof (inst_declared_inductive _ mdecl ind idecl (ren f) hΣ) as hi. *)
+(*   forward hi by assumption. rewrite <- hi. *)
+(*   eapply instantiate_params_rename with (f := f) in eity ; auto. *)
+(*   rewrite -> ind_type_map. *)
+(*   rewrite firstn_map. *)
+(*   lazymatch type of eity with *)
+(*   | ?t = _ => *)
+(*     lazymatch goal with *)
+(*     | |- match ?t' with _ => _ end = _ => *)
+(*       replace t' with t ; revgoals *)
+(*     end *)
+(*   end. *)
+(*   { autorewrite with sigma. *)
+(*     rewrite <- !rename_inst. *)
+(*     now rewrite rename_subst_instance_constr. } *)
+(*   rewrite eity. *)
+(*   case_eq (destArity [] ity) ; *)
+(*     try solve [ intro bot ; rewrite bot in h ; discriminate h ]. *)
+(*   intros [args0 ?] ear. rewrite ear in h. *)
+(*   eapply inst_destArity with (σ := ren f) in ear as ear'. *)
+(*   simpl in ear'. *)
+(*   lazymatch type of ear' with *)
+(*   | ?t = _ => *)
+(*     lazymatch goal with *)
+(*     | |- match ?t' with _ => _ end = _ => *)
+(*       replace t' with t ; revgoals *)
+(*     end *)
+(*   end. *)
+(*   { autorewrite with sigma. reflexivity. } *)
+(*   rewrite ear'. *)
+(*   case_eq (destArity [] pty) ; *)
+(*     try solve [ intro bot ; rewrite bot in h ; discriminate h ]. *)
+(*   intros [args' s'] epty. rewrite epty in h. *)
+(*   eapply inst_destArity with (σ := ren f) in epty as epty'. *)
+(*   simpl in epty'. *)
+(*   lazymatch type of epty' with *)
+(*   | ?t = _ => *)
+(*     lazymatch goal with *)
+(*     | |- match ?t' with _ => _ end = _ => *)
+(*       replace t' with t ; revgoals *)
+(*     end *)
+(*   end. *)
+(*   { autorewrite with sigma. reflexivity. } *)
+(*   rewrite epty'. *)
+(*   case_eq (map_option_out (build_branches_type ind mdecl idecl (firstn npar args) u p)) ; *)
+(*     try solve [ intro bot ; rewrite bot in h ; discriminate h ]. *)
+(*   intros brtys ebrtys. rewrite ebrtys in h. *)
+(*   inversion h. subst. clear h. *)
+(*   eapply build_branches_type_rename with (f := f) in ebrtys as ebrtys'. *)
+(*   2: assumption. *)
+(*   lazymatch type of ebrtys' with *)
+(*   | ?t = _ => *)
+(*     lazymatch goal with *)
+(*     | |- match ?t' with _ => _ end = _ => *)
+(*       replace t' with t ; revgoals *)
+(*     end *)
+(*   end. *)
+(*   { f_equal. f_equal. unfold map_one_inductive_body. destruct idecl. *)
+(*     simpl. f_equal. *)
+(*     - autorewrite with sigma. *)
+(*       eapply inst_ext. intro j. *)
+(*       unfold ren, shiftn. simpl. *)
+(*       f_equal. f_equal. lia. *)
+(*     - clear. induction ind_ctors. 1: reflexivity. *)
+(*       simpl. unfold on_pi2. destruct a. simpl. *)
+(*       destruct p. simpl. f_equal. 2: easy. *)
+(*       f_equal. f_equal. *)
+(*       autorewrite with sigma. *)
+(*       eapply inst_ext. intro j. *)
+(*       unfold ren, Upn, shiftn, subst_consn. *)
+(*       rewrite arities_context_length. *)
+(*       destruct (Nat.ltb_spec j #|ind_bodies mdecl|). *)
+(*       + rewrite nth_error_idsn_Some. all: easy. *)
+(*       + rewrite nth_error_idsn_None. 1: auto. *)
+(*         unfold subst_compose, shiftk. simpl. *)
+(*         rewrite idsn_length. reflexivity. *)
+(*     - clear. induction ind_projs. 1: auto. *)
+(*       simpl. destruct a. unfold on_snd. simpl. *)
+(*       f_equal. 2: easy. *)
+(*       f_equal. autorewrite with sigma. *)
+(*       eapply inst_ext. intro j. *)
+(*       unfold Upn, Up, ren, shiftn, subst_cons, subst_consn, subst_compose, *)
+(*       shift, shiftk. *)
+(*       destruct j. *)
+(*       + simpl. reflexivity. *)
+(*       + simpl. *)
+(*         destruct (Nat.ltb_spec (S j) (S (context_assumptions (ind_params mdecl)))). *)
+(*         * rewrite nth_error_idsn_Some. 1: lia. *)
+(*           simpl. reflexivity. *)
+(*         * rewrite nth_error_idsn_None. 1: lia. *)
+(*           simpl. rewrite idsn_length. reflexivity. *)
+(*   } *)
+(*   rewrite ebrtys'. autorewrite with sigma. reflexivity. *)
+(* Qed. *)
+
+
+Lemma inst_subst_instance_constr :
+  forall u t σ,
+    (subst_instance_constr u t).[(subst_instance_constr u ∘ σ)%prog] =
+    subst_instance_constr u t.[σ].
+Proof.
+  intros u t σ.
+  induction t in σ |- * using term_forall_list_ind.
+  all: simpl. all: auto.
+  all: autorewrite with sigma.
+  all: rewrite ?map_map_compose ?compose_on_snd ?compose_map_def ?map_lenght.
+  all: try solve [ f_equal ; eauto ; solve_all ; eauto ].
+  - rewrite IHt1. f_equal. rewrite <- IHt2.
+    eapply inst_ext. intro i.
+    unfold Up, subst_compose, subst_cons.
+    destruct i.
+    + reflexivity.
+    + pose proof (shift_subst_instance_constr u (σ i) 0) as e.
+      autorewrite with sigma in e. rewrite e. reflexivity.
+  -  f_equal;auto.
+Admitted.
+
+Lemma map_vass_map_def_inst g l s :
+  (mapi (fun i (d : def term) => vass (dname d) (lift0 i (dtype d)))
+        (map (map_def (inst s) g) l)) =
+  (mapi (fun i d => map_decl (inst (⇑^i s)) d)
+        (mapi (fun i (d : def term) => vass (dname d) (lift0 i (dtype d))) l)).
+Proof.
+  rewrite mapi_mapi mapi_map. apply mapi_ext.
+  intros. unfold map_decl, vass; simpl; f_equal.
+  rewrite !lift0_inst.
+  autorewrite with sigma.
+  rewrite shiftn_consn_idsn. reflexivity.
+Qed.
+
+Lemma inst_fix_context:
+  forall (mfix : list (def term)) s,
+    fix_context (map (map_def (inst s) (inst (⇑^#|mfix| s))) mfix) =
+    inst_context s (fix_context mfix).
+Proof.
+  intros mfix s. unfold fix_context.
+  rewrite map_vass_map_def_inst rev_mapi.
+  fold (fix_context mfix).
+  rewrite (inst_context_alt s (fix_context mfix)).
+   now rewrite mapi_length fix_context_length.
+Qed.
+
+Section Sigma.
+
+Context `{checker_flags}.
+
+(* Well-typedness of a substitution *)
+
+Definition well_subst Σ (Γ : context) σ (Δ : context) :=
+  forall x decl,
+    nth_error Γ x = Some decl ->
+    Σ ;;; Δ |- σ x : ((lift0 (S x)) (decl_type decl)).[ σ ] ×
+    (forall b,
+        decl.(decl_body) = Some b ->
+        σ x = b.[⇑^(S x) σ]
+    ).
+
+Notation "Σ ;;; Δ ⊢ σ : Γ" :=
+  (well_subst Σ Γ σ Δ) (at level 50, Δ, σ, Γ at next level).
+
+Lemma well_subst_Up :
+  forall Σ Γ Δ σ na A,
+    wf_local Σ (Δ ,, vass na A.[σ]) ->
+    Σ ;;; Δ ⊢ σ : Γ ->
+    Σ ;;; Δ ,, vass na A.[σ] ⊢ ⇑ σ : Γ ,, vass na A.
+Proof.
+  intros Σ Γ Δ σ na A hΔ h [|n] decl e.
+  - simpl in *. inversion e. subst. clear e. simpl.
+    split.
+    + eapply meta_conv.
+      * econstructor ; auto.
+        reflexivity.
+      * simpl.
+        autorewrite with sigma.
+        eapply inst_ext. intro i.
+        unfold subst_compose.
+        eapply inst_ext. intro j.
+        unfold shift, ren. reflexivity.
+    + intros b e. discriminate.
+  - simpl in *.
+    specialize (h _ _ e) as [h1 h2].
+    split.
+Admitted.
+
+Lemma well_subst_Up' :
+  forall Σ Γ Δ σ na t A,
+    wf_local Σ (Δ ,, vdef na t.[σ] A.[σ]) ->
+    Σ ;;; Δ ⊢ σ : Γ ->
+    Σ ;;; Δ ,, vdef na t.[σ] A.[σ] ⊢ ⇑ σ : Γ ,, vdef na t A.
+Proof.
+  intros Σ Γ Δ σ na t A wf h [|n] decl e.
+  - simpl in *. inversion e. subst. clear e. simpl.
+    rewrite lift_rename. rewrite rename_inst.
+    autorewrite with sigma.
+    split.
+    + eapply meta_conv.
+      * econstructor; auto; reflexivity.
+      * rewrite lift0_inst /=.
+        now autorewrite with sigma.
+    + intros b [= ->].
+      (* well-subst is ill-definied it should allow  let-preservation *)
+      admit.
+
+  - simpl in *.
+    specialize (h _ _ e).
+Admitted.
+
+(* (* Could be more precise *) *)
+(* Lemma instantiate_params_subst_length : *)
+(*   forall params pars s t s' t', *)
+(*     instantiate_params_subst params pars s t = Some (s', t') -> *)
+(*     #|params| >= #|pars|. *)
+(* Proof. *)
+(*   intros params pars s t s' t' h. *)
+(*   induction params in pars, s, t, s', t', h |- *. *)
+(*   - cbn in h. destruct pars. all: try discriminate. auto. *)
+(*   - cbn in h. destruct (decl_body a). *)
+(*     + destruct t. all: try discriminate. *)
+(*       cbn. eapply IHparams in h. lia. *)
+(*     + destruct t. all: try discriminate. *)
+(*       destruct pars. 1: discriminate. *)
+(*       cbn. eapply IHparams in h. lia. *)
+(* Qed. *)
+
+(* Lemma instantiate_params_length : *)
+(*   forall params pars T T', *)
+(*     instantiate_params params pars T = Some T' -> *)
+(*     #|params| >= #|pars|. *)
+(* Proof. *)
+(*   intros params pars T T' e. *)
+(*   unfold instantiate_params in e. *)
+(*   case_eq (instantiate_params_subst (List.rev params) pars [] T) ; *)
+(*     try solve [ intro bot ; rewrite bot in e ; discriminate e ]. *)
+(*   intros [s' t'] e'. rewrite e' in e. inversion e. subst. clear e. *)
+(*   eapply instantiate_params_subst_length in e'. *)
+(*   rewrite List.rev_length in e'. assumption. *)
+(* Qed. *)
+
+Lemma type_inst :
+  forall Σ Γ Δ σ t A,
+    wf Σ.1 ->
+    wf_local Σ Δ ->
+    Σ ;;; Δ ⊢ σ : Γ ->
+    Σ ;;; Γ |- t : A ->
+    Σ ;;; Δ |- t.[σ] : A.[σ].
+Proof.
+  intros Σ Γ Δ σ t A hΣ hΔ hσ h.
+  revert Σ hΣ Γ t A h Δ σ hΔ hσ.
+  apply (typing_ind_env (fun Σ Γ t T => forall Δ σ,
+    wf_local Σ Δ ->
+    Σ ;;; Δ ⊢ σ : Γ ->
+    Σ ;;; Δ |- t.[σ] : T.[σ]
+  ) (fun Σ Γ wfΓ => forall Δ σ, wf_local Σ Δ ->    Σ ;;; Δ ⊢ σ : Γ ->
+      wf_local Σ Δ)).
+  - intros Σ wfΣ Γ wfΓ. auto.
+    
+  - intros Σ wfΣ Γ wfΓ n decl e X Δ σ hΔ hσ. simpl.
+    eapply hσ. assumption.
+  - intros Σ wfΣ Γ wfΓ l X H0 Δ σ hΔ hσ. simpl.
+    econstructor. all: assumption.
+  - intros Σ wfΣ Γ wfΓ na A B s1 s2 X hA ihA hB ihB Δ σ hΔ hσ.
+    autorewrite with sigma. simpl.
+    econstructor.
+    + eapply ihA ; auto.
+    + eapply ihB.
+      * econstructor ; auto.
+        eexists. eapply ihA ; auto.
+      * eapply well_subst_Up. 2: assumption.
+        econstructor ; auto.
+        eexists. eapply ihA. all: auto.
+  - intros Σ wfΣ Γ wfΓ na A t s1 bty X hA ihA ht iht Δ σ hΔ hσ.
+    autorewrite with sigma.
+    econstructor.
+    + eapply ihA ; auto.
+    + eapply iht.
+      * econstructor ; auto.
+        eexists. eapply ihA ; auto.
+      * eapply well_subst_Up. 2: assumption.
+        constructor. 1: assumption.
+        eexists. eapply ihA. all: auto.
+  - intros Σ wfΣ Γ wfΓ na b B t s1 A X hB ihB hb ihb ht iht Δ σ hΔ hσ.
+    autorewrite with sigma.
+    econstructor.
+    + eapply ihB. all: auto.
+    + eapply ihb. all: auto.
+    + eapply iht.
+      * econstructor. all: auto.
+        -- eexists. eapply ihB. all: auto.
+        -- simpl. eapply ihb. all: auto.
+      * eapply well_subst_Up'; try assumption.
+        constructor; auto.
+        ** exists s1. apply ihB; auto.
+        ** apply ihb; auto.  
+  - intros Σ wfΣ Γ wfΓ t na A B s u X hty ihty ht iht hu ihu Δ σ hΔ hσ.
+    autorewrite with sigma.
+    econstructor.
+    * specialize (ihty _ _ hΔ hσ).
+      simpl in ihty. eapply meta_conv_term; [eapply ihty|].
+      now rewrite up_Up.
+    * specialize (iht _ _ hΔ hσ).
+      simpl in iht. eapply meta_conv; [eapply iht|].
+      now rewrite up_Up.
+    * eapply ihu; auto.
+  - intros Σ wfΣ Γ wfΓ cst u decl X X0 isdecl hconst Δ σ hΔ hσ.
+    autorewrite with sigma. simpl.
+    eapply meta_conv; [econstructor; eauto|].
+    eapply declared_constant_closed_type in isdecl; eauto.
+    rewrite inst_closed0; auto.
+    now rewrite closedn_subst_instance_constr.
+  - intros Σ wfΣ Γ wfΓ ind u mdecl idecl isdecl X X0 hconst Δ σ hΔ hσ.
+    eapply meta_conv; [econstructor; eauto|].
+    eapply declared_inductive_closed_type in isdecl; eauto.
+    rewrite inst_closed0; auto.
+    now rewrite closedn_subst_instance_constr.
+  - intros Σ wfΣ Γ wfΓ ind i u mdecl idecl cdecl isdecl X X0 hconst Δ σ hΔ hσ.
+    eapply meta_conv; [econstructor; eauto|].
+    eapply declared_constructor_closed_type in isdecl; eauto.
+    rewrite inst_closed0; eauto.
+  - intros Σ wfΣ Γ wfΓ ind u npar p c brs args mdecl idecl isdecl X X0 a pars
+           ps pty htoc X1 ihp H2 X3 notcoind ihc btys H3 ihbtys Δ σ hΔ hσ.
+    autorewrite with sigma. simpl.
+    rewrite map_app. simpl.
+    rewrite map_skipn.
+    (* eapply types_of_case_inst with (σ := σ) in htoc. all: try eassumption. *)
+    eapply type_Case.
+    + eassumption.
+    + assumption.
+    + admit.
+    + simpl. eapply ihp. all: auto.
+    + eassumption.
+    + specialize (ihc _ _ hΔ hσ). autorewrite with sigma in ihc.
+      eapply ihc.
+    + admit.
+    + admit.
+    + admit. 
+  - intros Σ wfΣ Γ wfΓ p c u mdecl idecl pdecl isdecl args X X0 hc ihc e ty
+           Δ σ hΔ hσ.
+    simpl.
+    eapply meta_conv; [econstructor|].
+    * eauto.
+    * specialize (ihc _ _ hΔ hσ).
+      rewrite inst_mkApps in ihc. eapply ihc.
+    * now rewrite map_length.
+    * autorewrite with sigma.
+      eapply declared_projection_closed in isdecl; auto.
+      admit.
+  - intros Σ wfΣ Γ wfΓ mfix n decl types H0 H1 X ihmfix Δ σ hΔ hσ.
+    autorewrite with sigma.
+    admit.
+  - intros Σ wfΣ Γ wfΓ mfix n decl types H0 X X0 ihmfix Δ σ hΔ hσ.
+    autorewrite with sigma.
+    admit.
+  - intros Σ wfΣ Γ wfΓ t A B X hwf ht iht hB ihB hcu Δ σ hΔ hσ.
+    eapply type_Cumul.
+    + eapply iht. all: auto.
+    + eapply ihB. all: auto.
+    + admit.
+Admitted.
