pcuic/theories/PCUICRename.v
@@ -1,0 +1,1401 @@
+(* Distributed under the terms of the MIT license. *)
+From Coq Require Import Morphisms.
+From MetaCoq.Template Require Import config utils.
+From MetaCoq.PCUIC Require Import PCUICAst PCUICAstUtils PCUICCases PCUICInduction
+  PCUICLiftSubst PCUICUnivSubst
+  PCUICTyping PCUICClosed PCUICEquality PCUICWeakeningEnv
+  PCUICSigmaCalculus.
+
+Require Import ssreflect ssrbool.
+From Equations Require Import Equations.
+Require Import Equations.Prop.DepElim.
+Set Equations With UIP.
+
+(** * Type preservation for σ-calculus operations *)
+
+Open Scope sigma_scope.
+Set Keyed Unification.
+
+Set Default Goal Selector "!".
+
+Lemma rename_mkApps :
+  forall f t l,
+    rename f (mkApps t l) = mkApps (rename f t) (map (rename f) l).
+Proof.
+  intros f t l.
+  autorewrite with sigma. f_equal.
+Qed.
+
+Lemma rename_subst_instance_constr :
+  forall u t f,
+    rename f (subst_instance_constr u t) = subst_instance_constr u (rename f t).
+Proof.
+  intros u t f.
+  induction t in f |- * using term_forall_list_ind.
+  all: try solve [
+    simpl ;
+    rewrite ?IHt ?IHt1 ?IHt2 ;
+    easy
+  ].
+  - simpl. f_equal. induction X.
+    + reflexivity.
+    + simpl. f_equal ; easy.
+  - simpl. rewrite IHt. f_equal.
+    * rewrite /rename_predicate !map_predicate_map_predicate.
+      solve_all.
+    * induction X0.
+      + reflexivity.
+      + simpl. f_equal. 2: easy.
+        destruct x. unfold map_branch. simpl in *.
+        easy.
+  - simpl. f_equal.
+    rewrite map_length.
+    generalize #|m|. intro k.
+    induction X. 1: reflexivity.
+    destruct p, x. unfold map_def in *.
+    simpl in *. f_equal. all: easy.
+  - simpl. f_equal.
+    rewrite map_length.
+    generalize #|m|. intro k.
+    induction X. 1: reflexivity.
+    destruct p, x. unfold map_def in *.
+    simpl in *. f_equal. all: easy.
+Qed.
+
+Definition rename_context f (Γ : context) : context :=
+  fold_context (fun i => rename (shiftn i f)) Γ.
+
+Definition rename_decl f d := map_decl (rename f) d.
+
+Lemma rename_context_length :
+  forall σ Γ,
+    #|rename_context σ Γ| = #|Γ|.
+Proof.
+  intros σ Γ. unfold rename_context.
+  apply fold_context_length.
+Qed.
+Hint Rewrite rename_context_length : sigma wf.
+
+Lemma rename_context_snoc0 :
+  forall f Γ d,
+    rename_context f (d :: Γ) =
+    rename_context f Γ ,, rename_decl (shiftn #|Γ| f) d.
+Proof.
+  intros f Γ d.
+  unfold rename_context. now rewrite fold_context_snoc0. 
+Qed.
+Hint Rewrite rename_context_snoc0 : sigma.
+
+Lemma rename_context_snoc r Γ d : rename_context r (Γ ,, d) = rename_context r Γ ,, map_decl (rename (shiftn #|Γ| r)) d.
+Proof.
+  unfold snoc. apply rename_context_snoc0.
+Qed.
+Hint Rewrite rename_context_snoc : sigma.
+
+Lemma rename_context_alt r Γ :
+  rename_context r Γ =
+  mapi (fun k' d => map_decl (rename (shiftn (Nat.pred #|Γ| - k') r)) d) Γ.
+Proof.
+  unfold rename_context. apply fold_context_alt.
+Qed.
+
+
+Lemma lift_renaming_0 k : ren (lift_renaming k 0) = ren (Nat.add k).
+Proof. reflexivity. Qed.
+
+Lemma ren_lift_renaming n k : ren (lift_renaming n k) =1 (⇑^k ↑^n).
+Proof.
+  unfold subst_compose. intros i.
+  simpl. rewrite -{1}(Nat.add_0_r k). unfold ren. rewrite - (shiftn_lift_renaming n k 0).
+  pose proof (ren_shiftn k (lift_renaming n 0) i).
+  change ((ren (shiftn k (lift_renaming n 0)) i) = ((⇑^k (↑^n)) i)).
+  rewrite -H. sigma. rewrite lift_renaming_0. reflexivity.
+Qed.
+
+Lemma rename_subst0 :
+  forall f l t,
+    rename f (subst0 l t) =
+    subst0 (map (rename f) l) (rename (shiftn #|l| f) t).
+Proof.
+  intros f l t.
+  autorewrite with sigma.
+  eapply inst_ext. intro i.
+  unfold ren, subst_consn, shiftn, subst_compose. simpl.
+  rewrite nth_error_map.
+  destruct (nth_error l i) eqn: e1.
+  - eapply nth_error_Some_length in e1 as hl.
+    destruct (Nat.ltb_spec i #|l|). 2: lia.
+    rewrite e1. simpl.
+    autorewrite with sigma. reflexivity.
+  - simpl. apply nth_error_None in e1 as hl.
+    destruct (Nat.ltb_spec i #|l|). 1: lia.
+    rewrite (iffRL (nth_error_None _ _)). 1: lia.
+    simpl. rewrite map_length. unfold ids.
+    f_equal. lia.
+Qed.
+
+Lemma rename_subst10 :
+  forall f t u,
+    rename f (t{ 0 := u }) = (rename (shiftn 1 f) t){ 0 := rename f u }.
+Proof.
+  intros f t u.
+  eapply rename_subst0.
+Qed.
+
+Lemma rename_context_nth_error :
+  forall f Γ i decl,
+    nth_error Γ i = Some decl ->
+    nth_error (rename_context f Γ) i =
+    Some (rename_decl (shiftn (#|Γ| - S i) f) decl).
+Proof.
+  intros f Γ i decl h.
+  induction Γ in f, i, decl, h |- *.
+  - destruct i. all: discriminate.
+  - destruct i.
+    + simpl in h. inversion h. subst. clear h.
+      rewrite rename_context_snoc0. simpl.
+      f_equal. f_equal. f_equal. lia.
+    + simpl in h. rewrite rename_context_snoc0. simpl.
+      eapply IHΓ. eassumption.
+Qed.
+
+Lemma rename_context_decl_body :
+  forall f Γ i body,
+    option_map decl_body (nth_error Γ i) = Some (Some body) ->
+    option_map decl_body (nth_error (rename_context f Γ) i) =
+    Some (Some (rename (shiftn (#|Γ| - S i) f) body)).
+Proof.
+  intros f Γ i body h.
+  destruct (nth_error Γ i) eqn: e. 2: discriminate.
+  simpl in h.
+  eapply rename_context_nth_error with (f := f) in e. rewrite e. simpl.
+  destruct c as [na bo ty]. simpl in h. inversion h. subst.
+  simpl. reflexivity.
+Qed.
+
+Lemma map_vass_map_def g l r :
+  (mapi (fun i (d : def term) => vass (dname d) (lift0 i (dtype d)))
+        (map (map_def (rename r) g) l)) =
+  (mapi (fun i d => map_decl (rename (shiftn i r)) d)
+        (mapi (fun i (d : def term) => vass (dname d) (lift0 i (dtype d))) l)).
+Proof.
+  rewrite mapi_mapi mapi_map. apply mapi_ext.
+  intros. unfold map_decl, vass; simpl; f_equal.
+  rewrite !lift_rename.
+  autorewrite with sigma. rewrite -ren_shiftn up_Upn.
+  rewrite shiftn_consn_idsn. reflexivity.
+Qed.
+
+Lemma rename_fix_context r :
+  forall (mfix : list (def term)),
+    fix_context (map (map_def (rename r) (rename (shiftn #|mfix| r))) mfix) =
+    rename_context r (fix_context mfix).
+Proof.
+  intros mfix. unfold fix_context.
+  rewrite map_vass_map_def rev_mapi.
+  fold (fix_context mfix).
+  rewrite (rename_context_alt r (fix_context mfix)).
+  unfold map_decl. now rewrite mapi_length fix_context_length.
+Qed.
+
+Section Renaming.
+
+Context `{checker_flags}.
+
+Lemma eq_term_upto_univ_rename Σ :
+  forall Re Rle napp u v f,
+    eq_term_upto_univ_napp Σ Re Rle napp u v ->
+    eq_term_upto_univ_napp Σ Re Rle napp (rename f u) (rename f v).
+Proof.
+  intros Re Rle napp u v f h.
+  induction u in v, napp, Rle, f, h |- * using term_forall_list_ind.
+  all: dependent destruction h.
+  all: try solve [
+    simpl ; constructor ; eauto
+  ].
+  - simpl. constructor.
+    induction X in a, args' |- *.
+    + inversion a. constructor.
+    + inversion a. subst. simpl. constructor.
+      all: eauto.
+  - simpl. constructor. all: eauto.
+    * rewrite /rename_predicate.
+      destruct X; destruct e as [? [? [ectx ?]]].
+      rewrite (All2_length ectx). red.
+      intuition auto; simpl; solve_all.
+    * induction X0 in a, brs' |- *.
+      + inversion a. constructor.
+      + inversion a. subst. simpl.
+        destruct X1 as [a0 e0]. rewrite (All2_length a0).
+        constructor.
+        ** unfold map_branch; simpl; intuition eauto.
+        ** eauto.
+  - simpl. constructor.
+    apply All2_length in a as e. rewrite <- e.
+    generalize #|m|. intro k.
+    induction X in mfix', a, f, k |- *.
+    + inversion a. constructor.
+    + inversion a. subst.
+      simpl. constructor.
+      * unfold map_def. intuition eauto.
+      * eauto.
+  - simpl. constructor.
+    apply All2_length in a as e. rewrite <- e.
+    generalize #|m|. intro k.
+    induction X in mfix', a, f, k |- *.
+    + inversion a. constructor.
+    + inversion a. subst.
+      simpl. constructor.
+      * unfold map_def. intuition eauto.
+      * eauto.
+Qed.
+
+(* Notion of valid renaming without typing information. *)
+Definition urenaming Γ Δ f :=
+  forall i decl,
+    nth_error Δ i = Some decl ->
+    ∑ decl',
+      nth_error Γ (f i) = Some decl' ×
+      rename f (lift0 (S i) decl.(decl_type))
+      = lift0 (S (f i)) decl'.(decl_type) ×
+      (forall b,
+         decl.(decl_body) = Some b ->
+         ∑ b',
+           decl'.(decl_body) = Some b' ×
+           rename f (lift0 (S i) b) = lift0 (S (f i)) b'
+      ).
+
+(* Definition of a good renaming with respect to typing *)
+Definition renaming Σ Γ Δ f :=
+  wf_local Σ Γ × urenaming Γ Δ f.
+
+Lemma rename_closedn :
+  forall f n t,
+    closedn n t ->
+    rename (shiftn n f) t = t.
+Proof.
+  intros f n t e.
+  autorewrite with sigma.
+  erewrite <- inst_closed with (σ := ren f) by eassumption.
+  eapply inst_ext. intro i.
+  unfold ren, shiftn, Upn, subst_consn, subst_compose, shift, shiftk.
+  rewrite idsn_length.
+  destruct (Nat.ltb_spec i n).
+  - rewrite nth_error_idsn_Some. all: auto.
+  - rewrite nth_error_idsn_None. 1: lia.
+    simpl. reflexivity.
+Qed.
+
+Lemma rename_closed_decl k f d : closed_decl k d -> map_decl (rename (shiftn k f)) d = d.
+Proof.
+  rewrite /closed_decl /map_decl.  
+  destruct d as [? [] ?] => /=.
+  - move/andP=> [] clt clty.
+    rewrite !rename_closedn //.
+  - move=> clt. rewrite !rename_closedn //.
+Qed.
+
+Lemma rename_closedn_ctx f n Γ : 
+  closedn_ctx n Γ -> 
+  rename_context (shiftn n f) Γ = Γ.
+Proof.
+  unfold closedn_ctx, rename_context.
+  apply alli_fold_context.
+  intros. rewrite shiftn_add.
+  intros. apply rename_closed_decl.
+  now rewrite Nat.add_comm.
+Qed.
+
+Lemma rename_closedn_terms f n ts : 
+  forallb (closedn n) ts -> map (rename (shiftn n f)) ts = ts.
+Proof.
+  solve_all. now apply rename_closedn.
+Qed.
+
+Lemma rename_closed_extended_subst f Γ : 
+  closed_ctx Γ ->
+  map (rename (shiftn (context_assumptions Γ) f)) (extended_subst Γ 0) = extended_subst Γ 0. 
+Proof.
+  intros cl. apply rename_closedn_terms.
+  now apply (closedn_extended_subst_gen Γ 0 0).
+Qed.
+
+(* TODO MOVE *)
+Lemma rename_closed :
+  forall f t,
+    closed t ->
+    rename f t = t.
+Proof.
+  intros f t h.
+  replace (rename f t) with (rename (shiftn 0 f) t).
+  - apply rename_closedn. assumption.
+  - autorewrite with sigma. eapply inst_ext. intro i.
+    unfold ren, shiftn. simpl.
+    f_equal. f_equal. lia.
+Qed.
+
+(* TODO MOVE *)
+Lemma declared_constant_closed_body :
+  forall Σ cst decl body,
+    wf Σ ->
+    declared_constant Σ cst decl ->
+    decl.(cst_body) = Some body ->
+    closed body.
+Proof.
+  intros Σ cst decl body hΣ h e.
+  unfold declared_constant in h.
+  eapply lookup_on_global_env in h. 2: eauto.
+  destruct h as [Σ' [wfΣ' decl']].
+  red in decl'. red in decl'.
+  destruct decl as [ty bo un]. simpl in *.
+  rewrite e in decl'.
+  now eapply subject_closed in decl'.
+Qed.
+
+Lemma rename_shiftn :
+  forall f k t,
+    rename (shiftn k f) (lift0 k t) = lift0 k (rename f t).
+Proof.
+  intros f k t.
+  autorewrite with sigma.
+  eapply inst_ext. intro i.
+  unfold ren, lift_renaming, shiftn, subst_compose. simpl.
+  destruct (Nat.ltb_spec (k + i) k); try lia.
+  unfold shiftk. lia_f_equal.
+Qed.
+
+Lemma urenaming_vass :
+  forall Γ Δ na A f,
+    urenaming Γ Δ f ->
+    urenaming (Γ ,, vass na (rename f A)) (Δ ,, vass na A) (shiftn 1 f).
+Proof.
+  intros Γ Δ na A f h. unfold urenaming in *.
+  intros [|i] decl e.
+  - simpl in e. inversion e. subst. clear e.
+    simpl. eexists. split. 1: reflexivity.
+    split.
+    + autorewrite with sigma.
+      eapply inst_ext. intro i.
+      unfold ren, lift_renaming, shiftn, subst_compose. simpl.
+      replace (i - 0) with i by lia. reflexivity.
+    + intros. discriminate.
+  - simpl in e. simpl.
+    replace (i - 0) with i by lia.
+    eapply h in e as [decl' [? [h1 h2]]].
+    eexists. split. 1: eassumption.
+    split.
+    + rewrite simpl_lift0. rewrite rename_shiftn. rewrite h1.
+      autorewrite with sigma.
+      eapply inst_ext. intro j.
+      unfold ren, lift_renaming, shiftn, subst_compose. simpl.
+      replace (i - 0) with i by lia.
+      reflexivity.
+    + intros b e'.
+      eapply h2 in e' as [b' [? hb]].
+      eexists. split. 1: eassumption.
+      rewrite simpl_lift0. rewrite rename_shiftn. rewrite hb.
+      autorewrite with sigma.
+      eapply inst_ext. intro j.
+      unfold ren, lift_renaming, shiftn, subst_compose. simpl.
+      replace (i - 0) with i by lia.
+      reflexivity.
+Qed.
+
+Lemma renaming_vass :
+  forall Σ Γ Δ na A f,
+    wf_local Σ (Γ ,, vass na (rename f A)) ->
+    renaming Σ Γ Δ f ->
+    renaming Σ (Γ ,, vass na (rename f A)) (Δ ,, vass na A) (shiftn 1 f).
+Proof.
+  intros Σ Γ Δ na A f hΓ [? h].
+  split. 1: auto.
+  eapply urenaming_vass. assumption.
+Qed.
+
+Lemma urenaming_vdef :
+  forall Γ Δ na b B f,
+    urenaming Γ Δ f ->
+    urenaming (Γ ,, vdef na (rename f b) (rename f B)) (Δ ,, vdef na b B) (shiftn 1 f).
+Proof.
+  intros Γ Δ na b B f h. unfold urenaming in *.
+  intros [|i] decl e.
+  - simpl in e. inversion e. subst. clear e.
+    simpl. eexists. split. 1: reflexivity.
+    split.
+    + autorewrite with sigma.
+      eapply inst_ext. intro i.
+      unfold ren, lift_renaming, shiftn, subst_compose. simpl.
+      replace (i - 0) with i by lia. reflexivity.
+    + intros b' [= <-].
+      simpl. eexists. split. 1: reflexivity.
+      autorewrite with sigma.
+      eapply inst_ext. intro i.
+      unfold ren, lift_renaming, shiftn, subst_compose. simpl.
+      replace (i - 0) with i by lia. reflexivity.
+  - simpl in e. simpl.
+    replace (i - 0) with i by lia.
+    eapply h in e as [decl' [? [h1 h2]]].
+    eexists. split. 1: eassumption.
+    split.
+    + rewrite simpl_lift0. rewrite rename_shiftn. rewrite h1.
+      autorewrite with sigma.
+      eapply inst_ext. intro j.
+      unfold ren, lift_renaming, shiftn, subst_compose. simpl.
+      replace (i - 0) with i by lia.
+      reflexivity.
+    + intros b0 e'.
+      eapply h2 in e' as [b' [? hb]].
+      eexists. split. 1: eassumption.
+      rewrite simpl_lift0. rewrite rename_shiftn. rewrite hb.
+      autorewrite with sigma.
+      eapply inst_ext. intro j.
+      unfold ren, lift_renaming, shiftn, subst_compose. simpl.
+      replace (i - 0) with i by lia.
+      reflexivity.
+Qed.
+
+Lemma renaming_vdef :
+  forall Σ Γ Δ na b B f,
+    wf_local Σ (Γ ,, vdef na (rename f b) (rename f B)) ->
+    renaming Σ Γ Δ f ->
+    renaming Σ (Γ ,, vdef na (rename f b) (rename f B)) (Δ ,, vdef na b B) (shiftn 1 f).
+Proof.
+  intros Σ Γ Δ na b B f hΓ [? h].
+  split. 1: auto.
+  eapply urenaming_vdef. assumption.
+Qed.
+
+Lemma urenaming_ext :
+  forall Γ Δ f g,
+    f =1 g ->
+    urenaming Δ Γ f ->
+    urenaming Δ Γ g.
+Proof.
+  intros Γ Δ f g hfg h.
+  intros i decl e.
+  specialize (h i decl e) as [decl' [h1 [h2 h3]]].
+  exists decl'. split ; [| split ].
+  - rewrite <- (hfg i). assumption.
+  - rewrite <- (hfg i). rewrite <- h2.
+    eapply rename_ext. intros j. symmetry. apply hfg.
+  - intros b hb. specialize (h3 b hb) as [b' [p1 p2]].
+    exists b'. split ; auto. rewrite <- (hfg i). rewrite <- p2.
+    eapply rename_ext. intros j. symmetry. apply hfg.
+Qed.
+
+Lemma urenaming_context :
+  forall Γ Δ Ξ f,
+    urenaming Δ Γ f ->
+    urenaming (Δ ,,, rename_context f Ξ) (Γ ,,, Ξ) (shiftn #|Ξ| f).
+Proof.
+  intros Γ Δ Ξ f h.
+  induction Ξ as [| [na [bo|] ty] Ξ ih] in Γ, Δ, f, h |- *.
+  - simpl. eapply urenaming_ext. 2: eassumption.
+    intros []. all: reflexivity.
+  - simpl. rewrite rename_context_snoc.
+    rewrite app_context_cons. simpl. unfold rename_decl. unfold map_decl. simpl.
+    eapply urenaming_ext.
+    2: eapply urenaming_vdef.
+    + intros [|i].
+      * reflexivity.
+      * unfold shiftn. simpl. replace (i - 0) with i by lia.
+        destruct (Nat.ltb_spec0 i #|Ξ|).
+        -- destruct (Nat.ltb_spec0 (S i) (S #|Ξ|)). all: easy.
+        -- destruct (Nat.ltb_spec0 (S i) (S #|Ξ|)). all: easy.
+    + eapply ih. assumption.
+  - simpl. rewrite rename_context_snoc.
+    rewrite app_context_cons. simpl. unfold rename_decl. unfold map_decl. simpl.
+    eapply urenaming_ext.
+    2: eapply urenaming_vass.
+    + intros [|i].
+      * reflexivity.
+      * unfold shiftn. simpl. replace (i - 0) with i by lia.
+        destruct (Nat.ltb_spec0 i #|Ξ|).
+        -- destruct (Nat.ltb_spec0 (S i) (S #|Ξ|)). all: easy.
+        -- destruct (Nat.ltb_spec0 (S i) (S #|Ξ|)). all: easy.
+    + eapply ih. assumption.
+Qed.
+
+Lemma rename_extended_subst f Γ k : 
+  map (rename (shiftn (context_assumptions Γ) f)) (extended_subst Γ k) =
+  extended_subst (rename_context (shiftn (context_assumptions Γ) f) Γ) k.
+Proof.
+  revert f k.
+  induction Γ as [|[na [] ?] Γ]; intros f k; cbn -[rename_context]; auto;
+    rewrite ?rename_context_snoc /=; len; rewrite ?IHΓ.
+  - f_equal. admit.
+  - 
+Admitted.
+
+Definition rename_branch f br := 
+  map_branch (rename (shiftn #|br.(bcontext)| f)) br.
+  
+  (* TODO MOVE *)
+Lemma rename_iota_red :
+  forall f pars args bctx br,
+    rename f (iota_red pars args bctx br) =
+    iota_red pars (map (rename f) args)
+       (rename_context f bctx)
+       (rename_branch f br).
+Proof.
+  intros f pars args bctx br.
+  unfold iota_red.
+  rewrite rename_subst0 map_skipn. f_equal.
+  rewrite /expand_lets /expand_lets_k.
+  rewrite rename_subst0. len.
+Admitted.
+  
+(* TODO MOVE *)
+Lemma isLambda_rename :
+  forall t f,
+    isLambda t ->
+    isLambda (rename f t).
+Proof.
+  intros t f h.
+  destruct t.
+  all: try discriminate.
+  simpl. reflexivity.
+Qed.
+
+(* TODO MOVE *)
+Lemma rename_unfold_fix :
+  forall mfix idx narg fn f,
+    unfold_fix mfix idx = Some (narg, fn) ->
+    unfold_fix (map (map_def (rename f) (rename (shiftn #|mfix| f))) mfix) idx
+    = Some (narg, rename f fn).
+Proof.
+  intros mfix idx narg fn f h.
+  unfold unfold_fix in *. rewrite nth_error_map.
+  case_eq (nth_error mfix idx).
+  2: intro neq ; rewrite neq in h ; discriminate.
+  intros d e. rewrite e in h.
+  inversion h. clear h.
+  simpl.
+  f_equal. f_equal.
+  rewrite rename_subst0. rewrite fix_subst_length.
+  f_equal.
+  unfold fix_subst. rewrite map_length.
+  generalize #|mfix| at 2 3. intro n.
+  induction n.
+  - reflexivity.
+  - simpl.
+    f_equal. rewrite IHn. reflexivity.
+Qed.
+
+(* TODO MOVE *)
+Lemma decompose_app_rename :
+  forall f t u l,
+    decompose_app t = (u, l) ->
+    decompose_app (rename f t) = (rename f u, map (rename f) l).
+Proof.
+  assert (aux : forall f t u l acc,
+    decompose_app_rec t acc = (u, l) ->
+    decompose_app_rec (rename f t) (map (rename f) acc) =
+    (rename f u, map (rename f) l)
+  ).
+  { intros f t u l acc h.
+    induction t in acc, h |- *.
+    all: try solve [ simpl in * ; inversion h ; reflexivity ].
+    simpl. simpl in h. specialize IHt1 with (1 := h). assumption.
+  }
+  intros f t u l.
+  unfold decompose_app.
+  eapply aux.
+Qed.
+
+(* TODO MOVE *)
+Lemma isConstruct_app_rename :
+  forall t f,
+    isConstruct_app t ->
+    isConstruct_app (rename f t).
+Proof.
+  intros t f h.
+  unfold isConstruct_app in *.
+  case_eq (decompose_app t). intros u l e.
+  apply decompose_app_rename with (f := f) in e as e'.
+  rewrite e'. rewrite e in h. simpl in h.
+  simpl.
+  destruct u. all: try discriminate.
+  simpl. reflexivity.
+Qed.
+
+(* TODO MOVE *)
+Lemma is_constructor_rename :
+  forall n l f,
+    is_constructor n l ->
+    is_constructor n (map (rename f) l).
+Proof.
+  intros n l f h.
+  unfold is_constructor in *.
+  rewrite nth_error_map.
+  destruct nth_error.
+  - simpl. apply isConstruct_app_rename. assumption.
+  - simpl. discriminate.
+Qed.
+
+(* TODO MOVE *)
+Lemma rename_unfold_cofix :
+  forall mfix idx narg fn f,
+    unfold_cofix mfix idx = Some (narg, fn) ->
+    unfold_cofix (map (map_def (rename f) (rename (shiftn #|mfix| f))) mfix) idx
+    = Some (narg, rename f fn).
+Proof.
+  intros mfix idx narg fn f h.
+  unfold unfold_cofix in *. rewrite nth_error_map.
+  case_eq (nth_error mfix idx).
+  2: intro neq ; rewrite neq in h ; discriminate.
+  intros d e. rewrite e in h.
+  inversion h.
+  simpl. f_equal. f_equal.
+  rewrite rename_subst0. rewrite cofix_subst_length.
+  f_equal.
+  unfold cofix_subst. rewrite map_length.
+  generalize #|mfix| at 2 3. intro n.
+  induction n.
+  - reflexivity.
+  - simpl.
+    f_equal. rewrite IHn. reflexivity.
+Qed.
+
+Definition rename_constructor_body mdecl f c := 
+  map_constructor_body #|mdecl.(ind_params)| #|mdecl.(ind_bodies)|
+   (fun k => rename (shiftn k f)) c.
+
+Lemma map2_set_binder_name_fold bctx f Γ :
+  #|bctx| = #|Γ| ->
+  map2 set_binder_name bctx (fold_context f Γ) = 
+  fold_context f (map2 set_binder_name bctx Γ).
+Proof.
+  intros hl.
+  rewrite !fold_context_alt mapi_map2 -{1}(map_id bctx).
+  rewrite -mapi_cst_map map2_mapi.
+  rewrite map2_length; len => //.
+  eapply map2i_ext => i x y.
+  rewrite hl.
+  destruct y; reflexivity.
+Qed.
+
+Lemma rename_subst :
+  forall f s n t,
+    rename (shiftn n f) (subst s n t) =
+    subst (map (rename f) s) n (rename (shiftn n (shiftn #|s| f)) t).
+Proof.
+  intros f s n t.
+  autorewrite with sigma.
+  eapply inst_ext. intro i. unfold Upn.
+  unfold ren, subst_consn, shiftn, subst_compose. simpl.
+  rewrite nth_error_map.
+  destruct (Nat.ltb_spec i n).
+  - rewrite idsn_lt //. simpl.
+    destruct (Nat.ltb_spec i n) => //. lia.
+  - rewrite nth_error_idsn_None //.
+    destruct (Nat.ltb_spec (i - n) #|s|).
+    * rewrite nth_error_idsn_None //; try lia.
+      len.
+      replace (n + (i - n) - n) with (i - n) by lia.
+      destruct nth_error eqn:hnth => /=.
+      ** sigma. apply inst_ext.
+        intros k. cbn.
+        elim: (Nat.ltb_spec (n + k) n); try lia.
+        intros. eapply nth_error_Some_length in hnth.
+        unfold shiftk. lia_f_equal.
+      ** eapply nth_error_None in hnth. lia.
+    * len.
+      replace (n + (#|s| + f (i - n - #|s|)) - n) with
+        (#|s| + f (i - n - #|s|)) by lia.
+      rewrite nth_error_idsn_None; try lia.
+      destruct nth_error eqn:hnth.
+      ** eapply nth_error_Some_length in hnth. lia.
+      ** simpl.
+        eapply nth_error_None in hnth.
+        destruct nth_error eqn:hnth'.
+        + eapply nth_error_Some_length in hnth'. lia.
+        + simpl. unfold shiftk.
+          case: Nat.ltb_spec; try lia.
+          intros. lia_f_equal.
+          assert (n + (i - n - #|s|) - n = (i - n - #|s|)) by lia.
+          rewrite H2. lia.
+Qed.
+
+Lemma rename_context_subst f s Γ : 
+  rename_context f (subst_context s 0 Γ) =
+  subst_context (map (rename f) s) 0 (rename_context (shiftn #|s| f) Γ).
+Proof.
+  rewrite !rename_context_alt !subst_context_alt.
+  rewrite !mapi_mapi. apply mapi_ext => i x.
+  rewrite /subst_decl !compose_map_decl.
+  apply map_decl_ext => t.
+  len.
+  generalize (Nat.pred #|Γ| - i).
+  intros.
+  now rewrite rename_subst.
+Qed.
+  
+Lemma rename_shiftnk :
+  forall f n k t,
+    rename (shiftn (n + k) f) (lift n k t) = lift n k (rename (shiftn k f) t).
+Proof.
+  intros f n k t.
+  autorewrite with sigma.
+  rewrite !ren_lift_renaming.
+  eapply inst_ext.
+  rewrite - !ren_shiftn up_Upn. rewrite Nat.add_comm. sigma.
+  rewrite !Upn_compose.
+  apply Upn_ext. now rewrite shiftn_consn_idsn.
+Qed.
+
+Lemma rename_context_lift f n k Γ : 
+  rename_context (shiftn (n + k) f) (lift_context n k Γ) =
+  lift_context n k (rename_context (shiftn k f) Γ).
+Proof.
+  rewrite !rename_context_alt !lift_context_alt.
+  rewrite !mapi_mapi. apply mapi_ext => i x.
+  rewrite /lift_decl !compose_map_decl.
+  apply map_decl_ext => t; len.
+  generalize (Nat.pred #|Γ| - i).
+  intros.
+  rewrite shiftn_add.
+  rewrite (Nat.add_comm n k) Nat.add_assoc Nat.add_comm.
+  now rewrite rename_shiftnk shiftn_add.
+Qed.
+
+Lemma rename_inds f ind pu bodies : map (rename f) (inds ind pu bodies) = inds ind pu bodies.
+Proof.
+  unfold inds.
+  induction #|bodies|; simpl; auto. f_equal.
+  apply IHn.
+Qed.
+
+
+Instance rename_context_ext : Proper (`=1` ==> Logic.eq ==> Logic.eq) rename_context.
+Proof.
+  intros f g Hfg x y ->.
+  apply fold_context_ext => i t.
+  now rewrite Hfg.
+Qed.
+
+Lemma rename_context_subst_instance_context f u Γ : 
+  rename_context f (subst_instance_context u Γ) = 
+  subst_instance_context u (rename_context f Γ).
+Proof. unfold rename_context.
+  rewrite fold_context_map //.
+  intros i x.
+  now rewrite rename_subst_instance_constr.
+Qed.
+
+Lemma fold_context_compose f g Γ : 
+  fold_context f (fold_context g Γ) = 
+  fold_context (fun i => f i ∘ g i) Γ.
+Proof.
+  rewrite !fold_context_alt mapi_mapi.
+  apply mapi_ext => i d.
+  rewrite compose_map_decl. apply map_decl_ext => t.
+  now len.
+Qed.
+
+Lemma rename_context_subst_k f s k Γ : 
+  rename_context (shiftn k f) (subst_context s k Γ) =
+  subst_context (map (rename f) s) k (rename_context (shiftn (k + #|s|) f) Γ).
+Proof.
+  rewrite /rename_context /subst_context.
+  rewrite !fold_context_compose.
+  apply fold_context_ext => i t.
+  rewrite shiftn_add.
+  now rewrite rename_subst !shiftn_add Nat.add_assoc.
+Qed.
+ 
+Lemma rename_cstr_args mdecl f cdecl : 
+  cstr_args (rename_constructor_body mdecl f cdecl) =
+  rename_context (shiftn (#|mdecl.(ind_params)| + #|ind_bodies mdecl|) f) (cstr_args cdecl).
+Proof. 
+  simpl. unfold rename_context.
+  apply fold_context_ext => i t.
+  now rewrite shiftn_add Nat.add_assoc.
+Qed.
+
+Lemma rename_case_branch_context_gen ind mdecl f p bctx cdecl :
+  closed_ctx (ind_params mdecl) ->
+  #|bctx| = #|cstr_args cdecl| ->
+  #|pparams p| = context_assumptions (ind_params mdecl) ->
+  rename_context f (case_branch_context ind mdecl p bctx cdecl) = 
+  case_branch_context ind mdecl (rename_predicate rename f p) bctx 
+    (rename_constructor_body mdecl f cdecl).
+Proof.
+  intros clpars. unfold case_branch_context, case_branch_context_gen.
+  rewrite rename_cstr_args.
+  cbn -[fold_context].
+  intros hlen hlen'.
+  rewrite map2_set_binder_name_fold //.
+  change (fold_context
+  (fun i : nat => rename (shiftn i (shiftn (ind_npars mdecl + #|ind_bodies mdecl|) f)))) with
+    (rename_context (shiftn (ind_npars mdecl + #|ind_bodies mdecl|) f)).
+  rewrite rename_context_subst. f_equal.
+  unfold id.
+  rewrite /expand_lets_ctx /expand_lets_k_ctx.
+  simpl. len.
+  rewrite rename_context_subst; len.
+  rewrite hlen'.
+  rewrite -{1}(context_assumptions_subst_instance_context (puinst p)).
+  rewrite rename_closed_extended_subst.
+  { now rewrite closedn_subst_instance_context. }
+  f_equal.
+  rewrite shiftn_add Nat.add_comm.
+  rewrite rename_context_lift. f_equal.
+  rewrite -rename_context_subst_instance_context.
+  rewrite rename_context_subst_k rename_inds. now len.
+Qed.
+
+Lemma rename_reln f ctx n acc :
+  forallb (closedn (n + #|ctx|)) acc ->
+  map (rename (shiftn (n + #|ctx|) f)) (reln acc n ctx) = 
+  reln acc n ctx.
+Proof.
+  induction ctx in n, acc |- *; simpl; auto.
+  - intros clacc. solve_all. now rewrite rename_closedn.
+  - intros clacc.
+    destruct a as [? [] ?].
+    * rewrite Nat.add_succ_r.
+      change (S (n + #|ctx|)) with (S n + #|ctx|).
+      rewrite Nat.add_1_r IHctx // /= -Nat.add_succ_r //.
+    * rewrite Nat.add_succ_r Nat.add_1_r. rewrite (IHctx (S n)) /= // -Nat.add_succ_r //.
+      simpl. rewrite clacc andb_true_r.
+      eapply Nat.ltb_lt. lia.
+Qed.
+
+Lemma rename_to_extended_list f ctx :
+  map (rename (shiftn #|ctx| f)) (to_extended_list ctx) = to_extended_list ctx.
+Proof.
+  unfold to_extended_list, to_extended_list_k.
+  now apply (rename_reln _ _ 0).
+Qed.
+
+Lemma closedn_ctx_expand_lets Γ Δ : 
+  closed_ctx (Γ ,,, Δ) ->
+  closedn_ctx (context_assumptions Γ) (expand_lets_ctx Γ Δ).
+Proof.
+  rewrite /expand_lets_ctx /expand_lets_k_ctx.
+  intros cl.
+  pose proof (closedn_ctx_subst (context_assumptions Γ) 0).
+  rewrite Nat.add_0_r in H0. apply: H0.
+  - simpl. len.
+    rewrite closedn_ctx_lift //.
+    rewrite closedn_ctx_app in cl. now move/andP: cl.
+  - apply (closedn_extended_subst_gen Γ 0 0).
+    rewrite closedn_ctx_app in cl.
+    now move/andP: cl => [].
+Qed.
+
+(* 
+Lemma rename_context_expand_lets_ctx k f Γ Δ :
+  k = context_assumptions Γ ->
+  rename_context (shiftn k f) (expand_lets_ctx Γ Δ) =
+  expand_lets_ctx (
+
+Lemma rename_context_expand_lets_ctx k f Γ Δ :
+  k = context_assumptions Γ ->
+  rename_context (shiftn k f) (expand_lets_ctx Γ Δ) =
+  expand_lets_ctx () *)
+
+Lemma rename_case_predicate_context Σ {wfΣ : wf Σ} ind mdecl idecl f p :
+  declared_inductive Σ ind mdecl idecl ->
+  wf_predicate mdecl idecl p ->
+  rename_context f (case_predicate_context ind mdecl idecl p) =
+  case_predicate_context ind mdecl idecl (rename_predicate rename f p).
+Proof.
+  intros decli wfp.
+  unfold case_predicate_context. simpl.
+  unfold id. unfold case_predicate_context_gen.
+  rewrite /rename_context.
+  rewrite -map2_set_binder_name_fold //.
+  - len. len. destruct wfp.
+    rewrite (Forall2_length H1) //.
+  - f_equal. rewrite fold_context_snoc0 /= /snoc.
+    f_equal.
+    * rewrite /map_decl /=. f_equal.
+      len. rewrite rename_mkApps /=. f_equal.
+      rewrite !map_app !map_map_compose. f_equal.
+      + solve_all.
+        eapply All_refl => x.
+        apply rename_shiftn.
+      + now rewrite rename_to_extended_list.
+    * rewrite -/(rename_context f _).
+      rewrite rename_context_subst rename_context_subst_instance_context.
+      f_equal. f_equal.
+      rewrite rename_closedn_ctx //.
+      pose proof (closedn_ctx_expand_lets (ind_params mdecl) (ind_indices idecl)
+        (declared_inductive_closed_pars_indices _ decli)).
+      rewrite (wf_predicate_length_pars wfp).
+      now rewrite (declared_minductive_ind_npars decli).
+Qed.
+
+Lemma rename_closed_constructor_body mdecl cdecl f : 
+  closed_constructor_body mdecl cdecl ->
+  rename_constructor_body mdecl f cdecl = cdecl.
+Proof.
+  rewrite /closed_constructor_body /rename_constructor_body /map_constructor_body.
+  move/andP=> [] /andP [] clctx clind clty.
+  destruct cdecl; cbn -[fold_context] in *; f_equal.
+  + move: clctx. unfold closed_ctx.
+    apply alli_fold_context => i d cldecl.
+    rewrite rename_closed_decl //.
+    red; rewrite -cldecl; lia_f_equal.
+  + solve_all. rewrite rename_closedn //.
+    red; rewrite -H0. lia_f_equal.
+  + now rewrite rename_closedn.
+Qed.
+
+Lemma rename_wf_predicate mdecl idecl f p :
+  wf_predicate mdecl idecl p ->
+  wf_predicate mdecl idecl (rename_predicate rename f p).
+Proof.
+  intros []. split.
+  - now len.
+  - apply H1.
+Qed.
+
+Lemma rename_wf_branch cdecl f br :
+  wf_branch cdecl br ->
+  wf_branch cdecl (rename_branch f br).
+Proof.
+  unfold wf_branch, wf_branch_gen. now simpl.
+Qed.
+
+Lemma Forall2_map_right {A B C} (P : A -> B -> Prop) (f : C -> B) (l : list A) (l' : list C) :
+  Forall2 P l (map f l') <-> Forall2 (fun x y => P x (f y)) l l'.
+Proof.
+  split; intros.
+  + eapply Forall2_map_inv. now rewrite map_id.
+  + rewrite -(map_id l). now eapply Forall2_map.  
+Qed.
+
+Lemma rename_wf_branches cdecl f brs :
+  wf_branches cdecl brs ->
+  wf_branches cdecl (map (rename_branch f) brs).
+Proof.
+  unfold wf_branches, wf_branches_gen.
+  intros h. solve_all. eapply Forall2_map_right.
+  solve_all.
+Qed.
+
+Lemma rename_predicate_set_pparams f p params :
+  rename_predicate rename f (set_pparams p params) = 
+  set_pparams (rename_predicate rename f p) (map (rename f) params).
+Proof. reflexivity. Qed.
+
+Lemma rename_predicate_set_preturn f p pret :
+  rename_predicate rename f (set_preturn p pret) = 
+  set_preturn (rename_predicate rename f p) (rename (shiftn #|pcontext p| f) pret).
+Proof. reflexivity. Qed.
+
+Lemma OnOne2All_All2_mix_left {A B} {P : B -> A -> A -> Type} {Q : B -> A -> Type} {i l l'} :
+  All2 Q i l -> OnOne2All P i l l' -> OnOne2All (fun i x y => (P i x y * Q i x)%type) i l l'.
+Proof.
+  intros a; induction 1; constructor; try inv a; intuition.
+Qed.
+
+Lemma red1_rename :
+  forall Σ Γ Δ u v f,
+    wf Σ ->
+    urenaming Δ Γ f ->
+    red1 Σ Γ u v ->
+    red1 Σ Δ (rename f u) (rename f v).
+Proof.
+  intros Σ Γ Δ u v f hΣ hf h.
+  induction h using red1_ind_all in f, Δ, hf |- *.
+  all: try solve [
+    simpl ; constructor ; eapply IHh ;
+    try eapply urenaming_vass ;
+    try eapply urenaming_vdef ;
+    assumption
+  ].
+  - simpl. rewrite rename_subst10. constructor.
+  - simpl. rewrite rename_subst10. constructor.
+  - simpl.
+    case_eq (nth_error Γ i).
+    2: intro e ; rewrite e in H0 ; discriminate.
+    intros decl e. rewrite e in H0. simpl in H0.
+    inversion H0. clear H0.
+    unfold urenaming in hf.
+    specialize hf with (1 := e).
+    destruct hf as [decl' [e' [hr hbo]]].
+    specialize hbo with (1 := H2).
+    destruct hbo as [body' [hbo' hr']].
+    rewrite hr'. constructor.
+    rewrite e'. simpl. rewrite hbo'. reflexivity.
+  - simpl. rewrite rename_mkApps. simpl.
+    rewrite rename_iota_red.
+    subst brctx.
+    rewrite rename_case_branch_context_gen.
+    * eapply declared_inductive_closed_params; eauto with pcuic.
+      eapply isdecl.
+    * now rewrite (Forall2_length H2).
+    * rewrite -(declared_minductive_ind_npars isdecl).
+      now eapply wf_predicate_length_pars.
+    * change (bcontext br) with (bcontext (rename_branch f br)).
+      epose proof (declared_constructor_closed _ isdecl).
+      rewrite rename_closed_constructor_body //.
+      eapply red_iota; eauto.
+      + rewrite nth_error_map H0 /= //.
+      + now apply rename_wf_predicate.
+  - rewrite 2!rename_mkApps. simpl.
+    econstructor.
+    + eapply rename_unfold_fix. eassumption.
+    + eapply is_constructor_rename. assumption.
+  - simpl.
+    rewrite 2!rename_mkApps. simpl.
+    eapply red_cofix_case.
+    eapply rename_unfold_cofix. eassumption.
+  - simpl. rewrite 2!rename_mkApps. simpl.
+    eapply red_cofix_proj.
+    eapply rename_unfold_cofix. eassumption.
+  - simpl. rewrite rename_subst_instance_constr.
+    econstructor.
+    + eassumption.
+    + rewrite rename_closed. 2: assumption.
+      eapply declared_constant_closed_body. all: eauto.
+  - simpl. rewrite rename_mkApps. simpl.
+    econstructor. rewrite nth_error_map. rewrite H0. reflexivity.
+  - simpl.
+    rewrite rename_predicate_set_pparams. econstructor.
+    simpl. eapply OnOne2_map. solve_all. red; eauto.
+  - simpl. rewrite rename_predicate_set_preturn.
+    eapply case_red_return; eauto.
+    + now apply rename_wf_predicate.
+    + simpl. apply IHh.
+      erewrite <-(case_predicate_context_length (p:=rename_predicate rename f p)); eauto.
+      2:{ now eapply rename_wf_predicate. }
+      rewrite - !rename_case_predicate_context; eauto.
+      len. now eapply urenaming_context.
+  - simpl.
+    eapply case_red_brs; eauto.
+    + now eapply rename_wf_predicate.
+    + now eapply rename_wf_branches.
+    + replace (ind_ctors idecl) with (map (rename_constructor_body mdecl f) (ind_ctors idecl)).
+      2:{ pose proof (declared_inductive_closed_constructors isdecl).
+          solve_all. now rewrite rename_closed_constructor_body. }
+      eapply OnOne2All_map_all. red in H1.
+      eapply Forall2_All2 in H1.
+      eapply OnOne2All_All2_mix_left in X; eauto. solve_all.
+      red; simpl. split; auto. rewrite -b0.
+      rewrite - rename_case_branch_context_gen; eauto.
+      * eapply (declared_inductive_closed_params isdecl).
+      * now apply wf_branch_length.
+      * rewrite -(declared_minductive_ind_npars isdecl).
+        now apply (wf_predicate_length_pars H0).
+      * eapply b1.
+        erewrite <-(case_branch_context_length b).
+        now eapply urenaming_context.
+  - simpl. constructor.
+    eapply OnOne2_map. solve_all. red. eauto.
+  - simpl.
+    apply OnOne2_length in X as hl. rewrite <- hl. clear hl.
+    generalize #|mfix0|. intro n.
+    constructor.
+    induction X.
+    + destruct p as [[p1 p2] p3]. inversion p3.
+      simpl. constructor. split.
+      * eapply p2. assumption.
+      * simpl. f_equal ; auto. f_equal ; auto.
+        f_equal. assumption.
+    + simpl. constructor. eapply IHX.
+  - simpl.
+    apply OnOne2_length in X as hl. rewrite <- hl. clear hl.
+    eapply fix_red_body.
+    Fail induction X using OnOne2_ind_l.
+    revert mfix0 mfix1 X.
+    refine (
+      OnOne2_ind_l _
+        (fun (L : mfixpoint term) (x y : def term) =>
+           (red1 Σ (Γ ,,, fix_context L) (dbody x) (dbody y)
+           × (forall (Δ0 : list context_decl) (f0 : nat -> nat),
+                 urenaming Δ0 (Γ ,,, fix_context L) f0 ->
+                 red1 Σ Δ0 (rename f0 (dbody x)) (rename f0 (dbody y))))
+           × (dname x, dtype x, rarg x) = (dname y, dtype y, rarg y)
+        )
+        (fun L mfix0 mfix1 o =>
+           OnOne2
+             (fun x y : def term =>
+                red1 Σ (Δ ,,, fix_context (map (map_def (rename f) (rename (shiftn #|L| f))) L)) (dbody x) (dbody y)
+                × (dname x, dtype x, rarg x) = (dname y, dtype y, rarg y))
+             (map (map_def (rename f) (rename (shiftn #|L| f))) mfix0)
+             (map (map_def (rename f) (rename (shiftn #|L| f))) mfix1)
+        )
+        _ _
+    ).
+    + intros L x y l [[p1 p2] p3].
+      inversion p3.
+      simpl. constructor. split.
+      * eapply p2. rewrite rename_fix_context.
+        rewrite <- fix_context_length.
+        eapply urenaming_context.
+        assumption.
+      * simpl. easy.
+    + intros L x l l' h ih.
+      simpl. constructor. eapply ih.
+  - simpl.
+    apply OnOne2_length in X as hl. rewrite <- hl. clear hl.
+    generalize #|mfix0|. intro n.
+    constructor.
+    induction X.
+    + destruct p as [[p1 p2] p3]. inversion p3.
+      simpl. constructor. split.
+      * eapply p2. assumption.
+      * simpl. f_equal ; auto. f_equal ; auto.
+        f_equal. assumption.
+    + simpl. constructor. eapply IHX.
+  - simpl.
+    apply OnOne2_length in X as hl. rewrite <- hl. clear hl.
+    eapply cofix_red_body.
+    Fail induction X using OnOne2_ind_l.
+    revert mfix0 mfix1 X.
+    refine (
+      OnOne2_ind_l _
+        (fun (L : mfixpoint term) (x y : def term) =>
+           (red1 Σ (Γ ,,, fix_context L) (dbody x) (dbody y)
+           × (forall (Δ0 : list context_decl) (f0 : nat -> nat),
+                 urenaming Δ0 (Γ ,,, fix_context L) f0 ->
+                 red1 Σ Δ0 (rename f0 (dbody x)) (rename f0 (dbody y))))
+           × (dname x, dtype x, rarg x) = (dname y, dtype y, rarg y)
+        )
+        (fun L mfix0 mfix1 o =>
+           OnOne2
+             (fun x y : def term =>
+                red1 Σ (Δ ,,, fix_context (map (map_def (rename f) (rename (shiftn #|L| f))) L)) (dbody x) (dbody y)
+                × (dname x, dtype x, rarg x) = (dname y, dtype y, rarg y))
+             (map (map_def (rename f) (rename (shiftn #|L| f))) mfix0)
+             (map (map_def (rename f) (rename (shiftn #|L| f))) mfix1)
+        )
+        _ _
+    ).
+    + intros L x y l [[p1 p2] p3].
+      inversion p3.
+      simpl. constructor. split.
+      * eapply p2. rewrite rename_fix_context.
+        rewrite <- fix_context_length.
+        eapply urenaming_context.
+        assumption.
+      * simpl. easy.
+    + intros L x l l' h ih.
+      simpl. constructor. eapply ih.
+Qed.
+
+Lemma cumul_rename :
+  forall Σ Γ Δ f A B,
+    wf Σ.1 ->
+    urenaming Δ Γ f ->
+    Σ ;;; Γ |- A <= B ->
+    Σ ;;; Δ |- rename f A <= rename f B.
+Proof.
+  intros Σ Γ Δ f A B hΣ hf h.
+  induction h.
+  - eapply cumul_refl. eapply eq_term_upto_univ_rename. assumption.
+  - eapply cumul_red_l.
+    + eapply red1_rename. all: try eassumption.
+    + assumption.
+  - eapply cumul_red_r.
+    + eassumption.
+    + eapply red1_rename. all: try eassumption.
+Qed.
+
+Lemma fix_guard_rename Σ Γ Δ mfix f :
+  renaming Σ Γ Δ f ->
+  let mfix' := map (map_def (rename f) (rename (shiftn (List.length mfix) f))) mfix in
+  fix_guard Σ Δ mfix ->
+  fix_guard Σ Γ mfix'.
+Admitted.
+
+Lemma cofix_guard_rename Σ Γ Δ mfix f :
+  renaming Σ Γ Δ f ->
+  let mfix' := map (map_def (rename f) (rename (shiftn (List.length mfix) f))) mfix in
+  cofix_guard Σ Δ mfix ->
+  cofix_guard Σ Γ mfix'.
+Admitted.
+
+Lemma typing_rename_prop : env_prop
+  (fun Σ Γ t A =>
+    forall Δ f,
+    renaming Σ Δ Γ f ->
+    Σ ;;; Δ |- rename f t : rename f A)
+   (fun Σ Γ _ => 
+    forall Δ f, 
+    renaming Σ Δ Γ f ->
+    wf_local Σ Δ).
+Proof.
+  apply typing_ind_env.
+  - now intros Σ wfΣ Γ wfΓ HΓ Δ f [hΔ hf].
+  
+  - intros Σ wfΣ Γ wfΓ n decl isdecl ihΓ Δ f [hΔ hf].
+    simpl. eapply hf in isdecl as h.
+    destruct h as [decl' [isdecl' [h1 h2]]].
+    rewrite h1. econstructor. all: auto.
+  - intros Σ wfΣ Γ wfΓ l X H0 Δ f [hΔ hf].
+    simpl. constructor. all: auto.
+  - intros Σ wfΣ Γ wfΓ na A B s1 s2 X hA ihA hB ihB Δ f hf.
+    simpl.
+    econstructor.
+    + eapply ihA. assumption.
+    + eapply ihB.
+      eapply renaming_vass. 2: auto.
+      constructor.
+      * destruct hf as [hΔ hf]. auto.
+      * simpl. exists s1. eapply ihA. assumption.
+  - intros Σ wfΣ Γ wfΓ na A t s1 B X hA ihA ht iht Δ f hf.
+    simpl. econstructor.
+    + eapply ihA. assumption.
+    + eapply iht.
+      eapply renaming_vass. 2: auto.
+      constructor.
+      * destruct hf as [hΔ hf]. auto.
+      * simpl. exists s1. eapply ihA. assumption.
+  - intros Σ wfΣ Γ wfΓ na b B t s1 A X hB ihB hb ihb ht iht Δ f hf.
+    simpl. econstructor.
+    + eapply ihB. assumption.
+    + eapply ihb. assumption.
+    + eapply iht.
+      eapply renaming_vdef. 2: auto.
+      constructor.
+      * destruct hf. assumption.
+      * simpl. eexists. eapply ihB. assumption.
+      * simpl. eapply ihb. assumption.
+  - intros Σ wfΣ Γ wfΓ t na A B s u X hty ihty ht iht hu ihu Δ f hf.
+    simpl. eapply meta_conv.
+    + eapply type_App.
+      * simpl in ihty. eapply ihty; eassumption.
+      * simpl in iht. eapply iht. assumption.
+      * eapply ihu. assumption.
+    + autorewrite with sigma. rewrite !subst1_inst. sigma.
+      eapply inst_ext. intro i.
+      unfold subst_cons, ren, shiftn, subst_compose. simpl.
+      destruct i.
+      * simpl. reflexivity.
+      * simpl. replace (i - 0) with i by lia.
+        reflexivity.
+  - intros Σ wfΣ Γ wfΓ cst u decl X X0 isdecl hconst Δ f hf.
+    simpl. eapply meta_conv.
+    + constructor. all: eauto.
+    + rewrite rename_subst_instance_constr. f_equal.
+      rewrite rename_closed. 2: auto.
+      eapply declared_constant_closed_type. all: eauto.
+  - intros Σ wfΣ Γ wfΓ ind u mdecl idecl isdecl X X0 hconst Δ σ hf.
+    simpl. eapply meta_conv.
+    + econstructor. all: eauto.
+    + rewrite rename_subst_instance_constr. f_equal.
+      rewrite rename_closed. 2: auto.
+      eapply declared_inductive_closed_type. all: eauto.
+  - intros Σ wfΣ Γ wfΓ ind i u mdecl idecl cdecl isdecl X X0 hconst Δ f hf.
+    simpl. eapply meta_conv.
+    + econstructor. all: eauto. 
+    + rewrite rename_closed. 2: reflexivity.
+      eapply declared_constructor_closed_type. all: eauto.
+  - intros Σ wfΣ Γ wfΓ ind u npar p c brs args mdecl idecl isdecl X X0 e
+           pars ps pty H1 X1 X2 H0 X3 X4 btys H2 X5 Δ f X6.
+    simpl.
+    rewrite rename_mkApps.
+    rewrite map_app. simpl.
+    rewrite map_skipn.
+    (* eapply types_of_case_inst with (σ := σ) in htoc. all: try eassumption. *)
+    (* eapply type_Case. *)
+    (* + eassumption. *)
+    (* + assumption. *)
+    (* + eapply ihp. all: auto. *)
+    (* + eassumption. *)
+    (* + admit. *)
+    (* + assumption. *)
+    (* + specialize (ihc _ _ hΔ hσ). autorewrite with sigma in ihc. *)
+    (*   eapply ihc. *)
+    (* + admit. *)
+    admit.
+  - intros Σ wfΣ Γ wfΓ p c u mdecl idecl pdecl isdecl args X X0 hc ihc e ty
+           Δ f hf.
+    simpl. eapply meta_conv.
+    + econstructor.
+      * eassumption.
+      * eapply meta_conv.
+        -- eapply ihc. assumption.
+        -- rewrite rename_mkApps. simpl. reflexivity.
+      * rewrite map_length. assumption.
+    + rewrite rename_subst0. simpl. rewrite map_rev. f_equal.
+      rewrite rename_subst_instance_constr. f_equal.
+      rewrite rename_closedn. 2: reflexivity.
+      eapply declared_projection_closed_type in isdecl. 2: auto.
+      rewrite List.rev_length. rewrite e. assumption.
+
+  - intros Σ wfΣ Γ wfΓ mfix n decl types H1 hdecl X ihmfixt ihmfixb wffix Δ f hf.
+    assert (hΔ' : wf_local Σ (Δ ,,, rename_context f (fix_context mfix))).
+    { rewrite - rename_fix_context.
+      apply PCUICWeakening.All_mfix_wf; auto; try apply hf.
+      eapply All_map, (All_impl ihmfixt).
+      intros x [s Hs]; exists s; intuition auto.
+      simpl. apply (b _ _ hf). }
+
+    simpl. eapply meta_conv.
+    + eapply type_Fix.
+      * eapply fix_guard_rename; eauto.
+      * rewrite nth_error_map. rewrite hdecl. simpl. reflexivity.
+      * apply hf.
+      * apply All_map, (All_impl ihmfixt).
+        intros x [s [Hs IHs]].
+        exists s. now apply IHs.
+      * apply All_map, (All_impl ihmfixb).
+        intros x [Hb IHb].
+        destruct x as [na ty bo rarg]. simpl in *.
+        rewrite rename_fix_context.
+        eapply meta_conv.
+        ++ apply (IHb (Δ ,,, rename_context f types) (shiftn #|mfix| f)).
+          split; auto. subst types. rewrite -(fix_context_length mfix).
+          apply urenaming_context; auto. apply hf.
+        ++ autorewrite with sigma. subst types. rewrite fix_context_length.
+          now rewrite -ren_shiftn up_Upn shiftn_consn_idsn.
+      * admit (* wf_fixpoint renaming *).
+    + reflexivity.
+
+  - intros Σ wfΣ Γ wfΓ mfix n decl types guard hdecl X ihmfixt ihmfixb wfcofix Δ f hf.
+    assert (hΔ' : wf_local Σ (Δ ,,, rename_context f (fix_context mfix))).
+    { rewrite -rename_fix_context.
+      apply PCUICWeakening.All_mfix_wf; auto; try apply hf.
+      eapply All_map, (All_impl ihmfixt).
+      intros x [s Hs]; exists s; intuition auto.
+      simpl. apply (b _ _ hf). }
+    simpl. eapply meta_conv.
+    + eapply type_CoFix; auto.
+      * eapply cofix_guard_rename; eauto.
+      * rewrite nth_error_map. rewrite hdecl. simpl. reflexivity.
+      * apply hf.
+      * apply All_map, (All_impl ihmfixt).
+        intros x [s [Hs IHs]].
+        exists s. now apply IHs.
+      * apply All_map, (All_impl ihmfixb).
+        intros x [Hb IHb].
+        destruct x as [na ty bo rarg]. simpl in *.
+        rewrite rename_fix_context.
+        eapply meta_conv.
+        ++ apply (IHb (Δ ,,, rename_context f types) (shiftn #|mfix| f)).
+            split; auto. subst types. rewrite -(fix_context_length mfix).
+            apply urenaming_context; auto. apply hf.
+        ++ autorewrite with sigma. subst types. rewrite fix_context_length.
+           now rewrite -ren_shiftn up_Upn shiftn_consn_idsn.
+      * admit.
+    + reflexivity.
+
+  - intros Σ wfΣ Γ wfΓ t A B X hwf ht iht htB ihB cum Δ f hf.
+    eapply type_Cumul.
+    + eapply iht. assumption.
+    + eapply ihB. assumption.
+    + eapply cumul_rename. all: try eassumption.
+      apply hf.
+Admitted.
+
+Lemma typing_rename :
+  forall Σ Γ Δ f t A,
+    wf Σ.1 ->
+    renaming Σ Δ Γ f ->
+    Σ ;;; Γ |- t : A ->
+    Σ ;;; Δ |- rename f t : rename f A.
+Proof.
+Admitted.
+  (* intros Σ Γ Δ f t A hΣ hf h.
+  revert Σ hΣ Γ t A h Δ f hf.
+  apply typing_rename_prop.
+Qed. *)
+
+End Renaming.
